# Context Free Grammar for Arithmetic Expressions

Operations considered - addition, subtraction, multiplication and division

The grammar:

```
A -> A + B | A - B | B
B -> B * C | B / C | C
C -> ( A ) | + C | - C | id
```

## LR(0) items

| 0                                                                                                                                                                         |
| ------------------------------------------------------------------------------------------------------------------------------------------------------------------------- |
| S' -> • A $                                                                                                                                                               |
| A -> • A + B <br/> A -> • A - B <br/> A -> • B <br/> B -> • B \* C <br/> B -> • B / C <br/> B -> • C <br/> C -> • ( A ) <br/> C -> • + C <br/> C -> • - C <br/> C -> • id |

| 1                                                              |
| -------------------------------------------------------------- |
| C -> + • C                                                     |
| C -> • ( A ) <br/> C -> • + C <br/> C -> • - C <br/> C -> • id |

| 2                                                              |
| -------------------------------------------------------------- |
| C -> - • C                                                     |
| C -> • ( A ) <br/> C -> • + C <br/> C -> • - C <br/> C -> • id |

| 3                                                                                                                                                                         |
| ------------------------------------------------------------------------------------------------------------------------------------------------------------------------- |
| C -> ( • A )                                                                                                                                                              |
| A -> • A + B <br/> A -> • A - B <br/> A -> • B <br/> B -> • B \* C <br/> B -> • B / C <br/> B -> • C <br/> C -> • ( A ) <br/> C -> • + C <br/> C -> • - C <br/> C -> • id |

| 4         |
| --------- |
| C -> id • |

| 5                                                 |
| ------------------------------------------------- |
| S' -> A • $ <br/> A -> A • + B <br/> A -> A • - B |

| 6                                               |
| ----------------------------------------------- |
| A -> B • <br/> B -> B • \* C <br/> B -> B • / C |

| 7        |
| -------- |
| B -> C • |

| 8                                                              |
| -------------------------------------------------------------- |
| B -> B \* • C                                                  |
| C -> • ( A ) <br/> C -> • + C <br/> C -> • - C <br/> C -> • id |

| 9                                                              |
| -------------------------------------------------------------- |
| B -> B / • C                                                   |
| C -> • ( A ) <br/> C -> • + C <br/> C -> • - C <br/> C -> • id |

| 10           |
| ------------ |
| B -> B / C • |

| 11            |
| ------------- |
| B -> B \* C • |

| 12          |
| ----------- |
| S' -> A $ • |

| 13                                                                                                                   |
| -------------------------------------------------------------------------------------------------------------------- |
| A -> A + • B                                                                                                         |
| B -> • B \* C <br/> B -> • B / C <br/> B -> • C <br/> C -> • ( A ) <br/> C -> • + C <br/> C -> • - C <br/> C -> • id |

| 14                                                                                                                   |
| -------------------------------------------------------------------------------------------------------------------- |
| A -> A - • B                                                                                                         |
| B -> • B \* C <br/> B -> • B / C <br/> B -> • C <br/> C -> • ( A ) <br/> C -> • + C <br/> C -> • - C <br/> C -> • id |

| 15                                                  |
| --------------------------------------------------- |
| A -> A - B • <br/> B -> B • \* C <br/> B -> B • / C |

| 16                                                  |
| --------------------------------------------------- |
| A -> A + B • <br/> B -> B • \* C <br/> B -> B • / C |

| 17                                                 |
| -------------------------------------------------- |
| C -> ( A • ) <br/> A -> A • + B <br/> A -> A • - B |

| 18           |
| ------------ |
| C -> ( A ) • |

| 19         |
| ---------- |
| C -> - C • |

| 20         |
| ---------- |
| C -> + C • |

## LR parsability

### LR(0)

States 6, 15 and 16 contain Shift- Reduce conflicts and hence make the grammar non LR(0)

### SLR(1)

Follow of A, B and C:
| |Follow|
|-|-|
|A| +&nbsp;&nbsp;&nbsp;&nbsp;-&nbsp;&nbsp;&nbsp;&nbsp;)&nbsp;&nbsp;&nbsp;&nbsp;$ |
|B| +&nbsp;&nbsp;&nbsp;&nbsp;-&nbsp;&nbsp;&nbsp;&nbsp;\*&nbsp;&nbsp;&nbsp;&nbsp;/&nbsp;&nbsp;&nbsp;&nbsp;)&nbsp;&nbsp;&nbsp;&nbsp;$|
|C| +&nbsp;&nbsp;&nbsp;&nbsp;-&nbsp;&nbsp;&nbsp;&nbsp;\*&nbsp;&nbsp;&nbsp;&nbsp;/&nbsp;&nbsp;&nbsp;&nbsp;)&nbsp;&nbsp;&nbsp;&nbsp;$|

Considering the Shift-Reduce conflicts caused by states 6, 15 and 16 - it can be noted that FOLLOW(A) does not contain \* or /, thus removing the conflicts according to SLR(1)

Hence the grammar is **SLR(1)**
